theories/invariant.v
@@ -4,14 +4,13 @@ Require Export diris.seplogic.
 Require Export diris.rtypesystem.
 Require Export diris.langlemmas.
 
-
-Definition conngraph := cgraph (V := object) (L := clabel).
+Definition conngraph := cgraph object clabel.
 Definition edges := gmap object clabel.
 
 Definition objects_match (g : conngraph) (es : list expr) (h : heap) : Prop. Admitted.
 
-Definition thread_inv (e : expr) (out_edges : edges) (in_edges : edges) : Prop :=
-    in_edges = ∅ ∧ holds (rtyped0 e UnitT) out_edges.
+Definition thread_inv (e : expr) (inlabels : list clabel) (outedges : edges) : Prop :=
+    inlabels = [] ∧ holds (rtyped0 e UnitT) outedges.
 
 
 
@@ -36,19 +35,19 @@ Definition bufs_typed (b1 b2 : option (list val)) (σ1 σ2 : option chan_type) :
   ∃ rest, buf_typed' b1 σ1 rest ∗
           buf_typed' b2 σ2 (dual rest).
 
-Inductive in_to_σ12 : edges -> option chan_type -> option chan_type -> Prop :=
-  | in_to_σ12_both o o' σ1 σ2 : in_to_σ12 {[ o := (true,σ1); o' := (false,σ2)]} (Some σ1) (Some σ2)
-  | in_to_σ12_left o σ1 : in_to_σ12 {[ o := (true,σ1) ]} (Some σ1) None
-  | in_to_σ12_right o σ2 : in_to_σ12 {[ o := (false,σ2) ]} None (Some σ2).
+Inductive in_to_σ12 : list clabel -> option chan_type -> option chan_type -> Prop :=
+  | in_to_σ12_both σ1 σ2 labs : labs ≡ₚ [(true,σ1);(false,σ2)] -> in_to_σ12 labs (Some σ1) (Some σ2)
+  | in_to_σ12_left σ1 : in_to_σ12 [(true,σ1)] (Some σ1) None
+  | in_to_σ12_right σ2 : in_to_σ12 [(false,σ2)] None (Some σ2).
 
-Definition chan_inv (b1 b2 : option (list val)) (in_edges : edges) (out_edges : edges) : Prop :=
-  ∃ σ1 σ2, in_to_σ12 in_edges σ1 σ2 ∧ holds (bufs_typed b1 b2 σ1 σ2) out_edges.
+Definition chan_inv (b1 b2 : option (list val)) (inlabels : list clabel) (outedges : edges) : Prop :=
+  ∃ σ1 σ2, in_to_σ12 inlabels σ1 σ2 ∧ holds (bufs_typed b1 b2 σ1 σ2) outedges.
 
 Definition threads_inv (g : conngraph) (es : list expr) :=
-  ∀ i e, es !! i = Some e -> thread_inv e (c_out g (Thread i)) (c_in g (Thread i)).
+  ∀ i e, es !! i = Some e -> thread_inv e (in_labels g (Thread i)) (out_edges g (Thread i)).
 
 Definition chans_inv (g : conngraph) (h : heap) :=
-  ∀ i, chan_inv (h !! (i,true)) (h !! (i,false)) (c_out g (Chan i)) (c_in g (Chan i)).
+  ∀ i, chan_inv (h !! (i,true)) (h !! (i,false)) (in_labels g (Chan i)) (out_edges g (Chan i)).
 
 Definition invariant (es : list expr) (h : heap) :=
   ∃ g : conngraph, cgraph_wf g ∧
@@ -95,6 +94,45 @@ Proof.
     simplify_eq.
     simplify_map_eq.
     rewrite !left_id_L in Hout.
+    assert (∃ g', cgraph_wf g' ∧
+      (∀ j, out_edges g' (Thread j) =
+        if decide (i = j)
+        then Σ1 ∪ {[Chan c.1 := (c.2, x)]}
+        else out_edges g (Thread j)) ∧
+      (∀ j, in_labels g' (Thread j) = in_labels g (Thread j)))
+    as (g' & Hwf' & Hthrout' & Hthrin').
+    {
+      admit.
+    }
+    exists g'.
+    split; eauto. split_and!.
+    + admit.
+    + unfold threads_inv. intros.
+      specialize (Hthrout' i0).
+      specialize (Hthrin' i0).
+      rewrite Hthrout'.
+      rewrite Hthrin'.
+      case_decide.
+      * subst. unfold thread_inv. split; eauto. rewrite list_lookup_insert in H2.
+        2: {
+          by eapply lookup_lt_Some.
+        }
+        simplify_eq.
+        assert (holds (rtyped0 (Val (ChanV c)) (ChanT x)) {[Chan c.1 := (c.2, x)]}).
+        {
+          simpl. apply exists_holds. eexists.
+          apply pure_sep_holds.
+          split; eauto.
+          apply own_holds. done.
+        }
+        pose proof (sep_combine _ _ _ _ Hctx H2) as HH.
+        assert (Σ1 ##ₘ {[Chan c.1 := (c.2, x)]}) by solve_map_disjoint.
+        specialize (HH H3).
+        eapply (holds_entails _ _ _ HH).
+        iIntros "[A B]".
+        iApply (ctx_subst0 with "A"). iFrame.
+      * apply Hthr. rewrite list_lookup_insert_ne in H2; eauto.
+    + intros ?. rewrite !lookup_insert_spec. admit.
     admit.
   - simpl in He.
     apply exists_holds in He as (?&He).
