theories/invtools.v
@@ -1,0 +1,56 @@
+Require Export diris.cgraph.
+Require Export diris.seplogic.
+
+Section invtools.
+  Context {V : Type}.
+  Context `{Countable V}.
+  Context {L : Type}.
+
+  Definition inv (g : cgraph V L) (f : V -> list L -> hProp V L) (h : V -> Prop) : Prop :=
+      cgraph_wf g ∧ ∀ v : V,
+      (v ∈ vertices g -> holds (f v (in_labels g v)) (out_edges g v)) ∧
+      (v ∉ vertices g -> h v).
+
+  Lemma inv_impl g f f' (h h' : V -> Prop) :
+    (∀ v ins, f v ins ⊢ f' v ins) ->
+    (∀ v, h v -> h' v) ->
+    inv g f h -> inv g f' h'.
+  Proof.
+    intros Hf Hh (Hg & HH).
+    split; first done.
+    intros v. split; last naive_solver.
+    intros Hv.
+    specialize (HH v) as [HH ?].
+    eauto using holds_entails.
+  Qed.
+
+  Lemma inv_init f (h : V -> Prop) :
+    (∀ v, h v) -> inv ∅ f h.
+  Proof.
+    intros HH.
+    split.
+    - apply empty_wf.
+    - set_solver.
+  Qed.
+
+  Lemma inv_singleton f (h : V -> Prop) (v : V) :
+    holds (f v []) ∅ ->
+    (∀ v', v' ≠ v -> h v') ->
+    inv {[ v := ∅ ]} f h.
+  Proof.
+    intros HH.
+    split.
+    - admit.
+    - intros v'. split.
+      + intros Hv. rewrite /vertices in Hv.
+        assert (v' = v) by set_solver. subst.
+        assert (in_labels ({[v := ∅]} : gmap V (gmap V L)) v = []) as HH1 by admit.
+        rewrite /out_edges. rewrite lookup_singleton. rewrite HH1. eauto.
+      + rewrite /vertices. set_solver.
+  Admitted.
+
+  Lemma inv_move f (h : V -> Prop) :
+    inv f h ->
+    (* We need to be able to express connectivity relationships here. *)
+    (* But we need that anyway for progress. *)
+    (* Think about how to handle that. *)
