theories/mapexcl.v
@@ -1,0 +1,124 @@
+From stdpp Require Export gmap.
+From iris.bi Require Export interface.
+From iris.algebra Require Import excl gmap auth.
+From iris.proofmode Require Export tactics.
+Require Export diris.util.
+
+
+Definition map_Excl `{Countable K} {V} (m : gmap K V) : gmap K (excl V) := Excl <$> m.
+
+Section map_Excl.
+  Context `{Countable K} {V : ofe} `{!LeibnizEquiv V}.
+  Implicit Type m : gmap K V.
+  Lemma map_Excl_valid m : ✓ (map_Excl m).
+  Proof. intros i. rewrite /map_Excl lookup_fmap. destruct (m !! i); done. Qed.
+  Lemma map_Excl_empty : map_Excl ∅ = (ε : gmap K (excl V)).
+  Proof. rewrite /map_Excl fmap_empty. done. Qed.
+  Lemma map_Excl_empty_inv Σ : map_Excl Σ = (∅ : gmap K (excl V)) -> Σ = ∅.
+  Proof.
+    rewrite /map_Excl. intros G. apply fmap_empty_inv in G. done.
+  Qed.
+
+  Lemma map_Excl_injective m1 m2 :
+    map_Excl m1 = map_Excl m2 -> m1 = m2.
+  Proof.
+    rewrite /map_Excl.
+    intros HH.
+  Admitted.
+  Lemma map_Excl_insert m k v :
+    map_Excl (<[ k := v ]> m) = <[ k := Excl v ]> $ map_Excl m.
+  Proof.
+    rewrite /map_Excl fmap_insert //.
+  Qed.
+  Lemma map_Excl_insert_op m k v :
+    m !! k = None ->
+    map_Excl (<[ k := v ]> m) = {[ k := Excl v ]} ⋅ map_Excl m.
+  Proof.
+    intros HH.
+    rewrite /map_Excl fmap_insert insert_singleton_op //
+            lookup_fmap HH //.
+  Qed.
+  Lemma map_Excl_union m1 m2 :
+    m1 ##ₘ m2 -> map_Excl (m1 ∪ m2) = map_Excl m1 ⋅ map_Excl m2.
+  Proof.
+    induction m1 using map_ind; intros; decompose_map_disjoint.
+    - by rewrite map_Excl_empty !left_id_L.
+    - assert ((m ∪ m2) !! i = None).
+      { rewrite lookup_union H0 H1 //. }
+      rewrite -insert_union_l !map_Excl_insert_op // IHm1 // assoc_L //.
+  Qed.
+  Lemma map_Excl_singleton_op_inv m me k x :
+    map_Excl m = {[ k := Excl x ]} ⋅ me ->
+    ∃ m', m = <[ k := x ]> m' ∧ me = map_Excl m' ∧ m' !! k = None.
+  Proof.
+    rewrite /map_Excl. intros HH.
+    exists (delete k m).
+    assert (m !! k = Some x).
+    { rewrite ->map_eq_iff in HH.
+      specialize (HH k).
+      revert HH. rewrite lookup_fmap lookup_op lookup_singleton.
+      case: (m!!k); case:(me!!k); simpl; intros; inversion HH. done. }
+    rewrite !map_eq_iff.
+    rewrite-> map_eq_iff in HH.
+    split_and!.
+    - intros i.
+      destruct (decide (k = i)); subst.
+      + rewrite lookup_insert //.
+      + rewrite lookup_insert_ne // lookup_delete_ne //.
+    - intros i.
+      specialize (HH i).
+      destruct (decide (k = i)); subst.
+      + rewrite lookup_fmap lookup_delete.
+        revert HH. rewrite !lookup_fmap lookup_op lookup_singleton H0 /=.
+        case: (me !! i); eauto.
+        intros a HH. inversion HH.
+      + rewrite lookup_fmap lookup_delete_ne //.
+        revert HH. rewrite lookup_fmap lookup_op lookup_singleton_ne //.
+        case: (me !! i); simpl; intros; rewrite HH //.
+    - rewrite lookup_delete //.
+  Qed.
+  Lemma map_Excl_union_inv m me1 me2 :
+    map_Excl m = me1 ⋅ me2 ->
+    ∃ m1 m2, m = m1 ∪ m2 ∧ me1 = map_Excl m1 ∧ me2 = map_Excl m2 ∧ m1 ##ₘ m2.
+  Proof.
+    revert m. induction me1 as [|k xe me1 Hx IH] using map_ind; intros m.
+    - rewrite left_id_L. intros <-.
+      exists ∅,m.
+      rewrite left_id_L map_Excl_empty. split_and!; solve_map_disjoint.
+    - rewrite insert_singleton_op // -assoc_L.
+      destruct xe as [x|].
+      + intros (m' & -> & ? & ?)%map_Excl_singleton_op_inv.
+        destruct (IH m') as (m1 & m2 & -> & -> & -> & ?); first done.
+        exists (<[ k := x]> m1),m2.
+        apply lookup_union_None in H1 as [].
+        repeat split.
+        * by rewrite insert_union_l.
+        * rewrite map_Excl_insert_op //.
+        * by apply map_disjoint_insert_l.
+      + intros Hm. assert (✓ (ExclBot : excl V)) as [].
+        eapply (singleton_valid k), (cmra_valid_op_l _ (me1 ⋅ me2)).
+        rewrite -Hm. apply map_Excl_valid.
+  Qed.
+  Lemma map_Excl_disjoint m1 m2 :
+    m1 ##ₘ m2 <-> map_Excl m1 ##ₘ map_Excl m2.
+  Proof.
+    split; first apply fmap_map_disjoint.
+    unfold map_Excl. intros G ?. specialize (G i).
+    rewrite !lookup_fmap in G.
+    destruct (m1 !! i),(m2 !! i); done.
+  Qed.
+End map_Excl.
+
+Lemma map_Excl_singleton `{Countable K} {V} (a : K) (b : V) :
+  map_Excl {[ a := b ]} = {[ a := Excl b ]}.
+Proof.
+  rewrite /map_Excl map_fmap_singleton //.
+Qed.
+Lemma map_Excl_singleton_inv `{Countable K} {V} a b (Σ : gmap K V) :
+  map_Excl Σ = {[ a := Excl b ]} -> Σ = {[ a := b ]}.
+Proof.
+  intros HH.
+  pose proof (fmap_singleton_inv _ _ _ _ HH).
+  destruct H0 as [? ->]. rewrite map_Excl_singleton in HH.
+  apply singleton_eq_iff in HH. destruct HH. simplify_eq. done.
+Qed.
